start on pop_seq, traces and pre_star_rule_cases

WPDS/WPDS.thy
@@ -142,6 +142,9 @@ type_synonym ('state, 'label, 'weight) w_transitions = "('state, 'label) transit
 
 type_synonym ('state, 'label, 'weight) w_transition_set = "('state, ('label list \<times> 'weight)) transition set"
 
+(* A final trace gives a list of pop_seqs followed by a list of automata transitions, where only the first has non-trivial weight.*)
+type_synonym ('ctr_loc, 'noninit, 'label) final_trace = "('ctr_loc, 'label) trace \<times> ('label \<times> 'noninit) list"
+
 \<comment> \<open>Embed a weighted automata into a monoidLTS. All non-zero transitions are added. The label is lifted to the list-monoid.\<close>
 definition wts_to_monoidLTS :: "(('state, 'label, 'weight::{dioid_one_zero,reverse_wqo}) w_transitions) \<Rightarrow> ('state, ('label list \<times> 'weight)) transition set" where
   "wts_to_monoidLTS ts = {(p, ([l],d), q) | p l d q. ts $ (p,l,q) = d \<and> d \<noteq> 0}"
@@ -202,6 +205,22 @@ notation monoid_star_relp ("(_)/ \<Midarrow> (_)/ \<Rightarrow>\<^sup>* (_)/" [9
 \<comment> \<open>Generalization of @{term PDS_with_P_automata.accepts} that computes the meet-over-all-paths in the W-automaton.\<close>
 definition accepts :: "(('ctr_loc, 'noninit, 'label) state, 'label, 'weight) w_transitions \<Rightarrow> ('ctr_loc, 'label) conf \<Rightarrow> 'weight" where
   "accepts ts \<equiv> \<lambda>(p,w). (\<Sum>{d | d q. q \<in> finals \<and> (Init p,(w,d),q) \<in> monoidLTS.monoid_star (wts_to_monoidLTS ts)})"
+
+definition pop_seq :: "'ctr_loc \<Rightarrow> 'label \<Rightarrow> 'ctr_loc \<Rightarrow> 'weight" where
+  "pop_seq p \<gamma> p' = \<Sum>{d. (p,[\<gamma>]) \<Midarrow>d\<Rightarrow>\<^sup>* (p',[])}"
+
+lemma "(pop_seq p \<gamma> p') \<le> \<Sum>{d. (p,\<gamma>#w) \<Midarrow>d\<Rightarrow>\<^sup>* (p',w)}"
+  using step_relp_def2[of p "\<gamma>#w" _ p' w]
+  apply simp
+  unfolding pop_seq_def
+  apply auto
+  oops
+
+lemma "(pop_seq p \<gamma> p') * (pop_seq p' \<gamma>' p'') \<le> \<Sum>{d. (p,[\<gamma>,\<gamma>']) \<Midarrow>d\<Rightarrow>\<^sup>* (p'',[])}"
+  unfolding pop_seq_def
+  apply simp
+  oops
+
 
 \<comment> \<open>Weighted pre-star rule updates the finfun of transition weights.\<close>
 inductive pre_star_rule :: "(('ctr_loc, 'noninit, 'label) state, 'label, 'weight) w_transitions saturation_rule" where 
@@ -282,6 +301,242 @@ lemma pre_star_saturation_exi:
   shows "\<exists>ts'. saturation pre_star_rule ts ts'"
   by (rule reverse_wqo_class_saturation_exi[of pre_star_rule ts])
      (auto simp add:pre_star_rule.simps pre_star_saturation_less)
+
+
+lemma wts_label_exist: "(p, w, q) \<in> wts_to_monoidLTS ts \<Longrightarrow> \<exists>l. fst w = [l]"
+  unfolding wts_to_monoidLTS_def by fastforce
+
+lemma wts_label_size: "(p, w, q) \<in> wts_to_monoidLTS ts \<Longrightarrow> size (fst w) = 1"
+  unfolding wts_to_monoidLTS_def by fastforce
+
+lemma wts_label_not_empty: "(p, w, q) \<in> wts_to_monoidLTS ts \<Longrightarrow> fst w \<noteq> []"
+  unfolding wts_to_monoidLTS_def by force
+
+lemma wts_label_d: "(p, ([l],d), q) \<in> wts_to_monoidLTS ts \<Longrightarrow> ts $ (p,l,q) = d"
+  unfolding wts_to_monoidLTS_def by blast
+
+lemma wts_label_d': "(p, w, q) \<in> wts_to_monoidLTS ts \<Longrightarrow> ts $ (p, hd(fst w), q) = snd w"
+  unfolding wts_to_monoidLTS_def by auto
+
+lemma mstar_wts_one: "(p, w, q) \<in> monoid_rtrancl (wts_to_monoidLTS ts) \<Longrightarrow> fst w = 1 \<Longrightarrow> snd w = 1"
+proof (induct rule: monoid_rtrancl.induct)
+  case (monoid_rtrancl_refl a)
+  then show ?case by (simp add: one_prod_def)
+next
+  case (monoid_rtrancl_into_rtrancl a w b l c)
+  from \<open>(b, l, c) \<in> wts_to_monoidLTS ts\<close> have "fst l \<noteq> []" using wts_label_not_empty by fast
+  then have \<open>fst (w \<cdot> l) \<noteq> []\<close> by (simp add: mult_prod_def times_list_def)
+  then show ?case by (simp add: monoid_rtrancl_into_rtrancl.prems one_list_def)
+qed
+lemma mstar_wts_empty_one: "(p, ([],d), q) \<in> monoid_rtrancl (wts_to_monoidLTS ts) \<Longrightarrow> d = 1"
+  using mstar_wts_one by (simp add: one_list_def, fastforce)
+
+lemma monoid_star_pop':
+  assumes "(p, w, q) \<in> monoid_rtrancl (wts_to_monoidLTS ts)"
+  assumes "fst w = []"
+  shows " p = q"
+  using assms
+proof (induct rule: monoid_rtrancl.induct)
+  case (monoid_rtrancl_refl a)
+  then show ?case by simp
+next
+  case (monoid_rtrancl_into_rtrancl a w b l c)
+  from \<open>(b, l, c) \<in> wts_to_monoidLTS ts\<close> have "fst l \<noteq> []" using wts_label_not_empty by fast
+  then have \<open>fst (w \<cdot> l) \<noteq> []\<close> by (simp add: mult_prod_def times_list_def)
+  then show ?case by (simp add: monoid_rtrancl_into_rtrancl.prems)
+qed
+lemma monoid_star_pop:
+  assumes "(Init p, (lbl w, d), q) \<in> monoidLTS.monoid_star (wts_to_monoidLTS ts)"
+  assumes "w = pop"
+  shows   "q = Init p \<and> d = 1"
+  using assms monoid_star_pop' by (auto simp add: one_list_def mstar_wts_empty_one) fastforce
+
+lemma monoid_star_swap':
+  assumes "(p, w, q) \<in> monoid_rtrancl (wts_to_monoidLTS ts)"
+  assumes "fst w = [l]"
+  shows "ts $ (p,l,q) = snd w"
+  using assms
+proof (induct rule: monoid_rtrancl.induct)
+  case (monoid_rtrancl_refl a)
+  then show ?case by (simp add: one_prod_def one_list_def)
+next
+  case (monoid_rtrancl_into_rtrancl a w b w' c)
+  then have "fst w = []" 
+    by (simp add: mult_prod_def times_list_def append_eq_Cons_conv wts_label_not_empty[of b w' c ts])
+  then show ?case 
+    using monoid_rtrancl_into_rtrancl.hyps monoid_rtrancl_into_rtrancl.prems
+          monoid_star_pop'[of a w b ts] mstar_wts_one[of a w b ts] wts_label_d'[of b w' c ts]
+    by (simp add: mult_prod_def one_list_def times_list_def)
+qed
+lemma monoid_star_swap:
+  assumes "(Init p, (lbl w, d), q) \<in> monoidLTS.monoid_star (wts_to_monoidLTS ts)"
+  assumes "w = swap l"
+  shows "ts $ (Init p,l,q) = d"
+  using assms monoid_star_swap' by fastforce
+
+lemma monoid_star_push':
+  assumes "(p, w, q) \<in> monoid_rtrancl (wts_to_monoidLTS ts)"
+  assumes "fst w = [l,l']"
+  shows "\<exists>q'. ts $ (p,l,q') * ts $ (q',l',q) = snd w"
+  using assms
+proof (induct rule: monoid_rtrancl.induct)
+  case (monoid_rtrancl_refl a)
+  then show ?case by (simp add: one_prod_def one_list_def)
+next
+  case (monoid_rtrancl_into_rtrancl a w b w' c)
+  then have "fst w = [l] \<and> fst w' = [l']" 
+    using wts_label_exist[of b w' c ts] 
+    by (auto simp add: times_list_def mult_prod_def)
+  then show ?case 
+    using monoid_rtrancl_into_rtrancl.hyps monoid_rtrancl_into_rtrancl.prems 
+          monoid_star_swap'[of a w b ts l] monoid_star_swap'[of b w' c ts l'] wts_label_d'[of b w' c ts]    
+    by (simp add: mult_prod_def) metis
+qed
+lemma monoid_star_push:
+  assumes "(Init p, (lbl w, d), q) \<in> monoidLTS.monoid_star (wts_to_monoidLTS ts)"
+  assumes "w = push l l'"
+  shows "\<exists>q'. ts $ (Init p,l,q') * ts $ (q',l',q) = d"
+  using assms monoid_star_push' by fastforce
+
+lemma pre_star_rule_cases:
+  assumes "(Init p, (lbl w, d), q) \<in> monoidLTS.monoid_star (wts_to_monoidLTS ts)"
+  shows "(w = pop \<and> q = Init p \<and> d = 1) \<or>                          
+         (\<exists>l. w = swap l \<and> ts $ (Init p,l,q) = d) \<or> 
+         (\<exists>l l'. w = push l l' \<and> (\<exists>q'. ts $ (Init p,l,q') * ts $ (q',l',q) = d))"
+proof (cases rule: operation.exhaust[of w])
+  case pop
+  then show ?thesis using monoid_star_pop[OF assms(1)] by simp
+next
+  case (swap l)
+  then show ?thesis using monoid_star_swap[OF assms(1)] by simp
+next
+  case (push l l')
+  then show ?thesis using monoid_star_push[OF assms(1)] by simp
+qed
+lemma pre_star_rule_exhaust:
+  assumes "(Init p, (lbl w, d), q) \<in> monoidLTS.monoid_star (wts_to_monoidLTS ts)"
+  assumes "q = Init p \<and> d = 1 \<Longrightarrow> P"
+  assumes "\<And>l. ts $ (Init p,l,q) = d \<Longrightarrow> P"
+  assumes "\<And>l l'. \<exists>q'. ts $ (Init p,l,q') * ts $ (q',l',q) = d \<Longrightarrow> P"
+  shows "P"
+  using pre_star_rule_cases[OF assms(1)] assms(2,3,4) by blast
+
+lemma pre_star_rule_update_is_Init:
+  assumes "pre_star_rule A A'"
+      and "A $ (p,\<gamma>,q) \<noteq> A' $ (p,\<gamma>,q)"
+    shows "is_Init p"
+  using assms unfolding pre_star_rule.simps
+  apply safe
+  subgoal for p' by (cases "p = Init p'", auto)
+  done
+lemma pre_star_rule_update_inits:
+  assumes "pre_star_rule A A'"
+      and "A $ (p,\<gamma>,q) \<noteq> A' $ (p,\<gamma>,q)"
+    shows "p \<in> inits"
+  using pre_star_rule_update_is_Init[OF assms] unfolding inits_def by simp
+
+lemma pre_star_rule_update_spec':
+  assumes "pre_star_rule A A'"
+      and "A $ (Init p,\<gamma>,q) \<noteq> A' $ (Init p,\<gamma>,q)"
+    shows "\<exists>d d' p' w. A' $ (Init p,\<gamma>,q) = A $ (Init p, \<gamma>, q) + d \<cdot> d' \<and> (p, \<gamma>) \<midarrow>d\<hookrightarrow> (p', w) \<and> (Init p', (lbl w, d'), q) \<in> monoid_rtrancl (wts_to_monoidLTS A) \<and> A $ (Init p, \<gamma>, q) + d \<cdot> d' \<noteq> A $ (Init p, \<gamma>, q)"
+  using assms unfolding pre_star_rule.simps
+  apply safe
+  subgoal for p' \<gamma>' _ _ _ _ q'
+    by (cases "(p,\<gamma>,q) = (p', \<gamma>',q')", auto)
+  done
+lemma pre_star_rule_update_spec:
+  assumes "pre_star_rule A A'"
+      and "A $ (p,\<gamma>,q) \<noteq> A' $ (p,\<gamma>,q)"
+    shows "\<exists>d d' p' w. A' $ (p,\<gamma>,q) = A $ (p, \<gamma>, q) + d \<cdot> d' \<and> (the_Ctr_Loc p, \<gamma>) \<midarrow>d\<hookrightarrow> (p', w) \<and> (Init p', (lbl w, d'), q) \<in> monoid_rtrancl (wts_to_monoidLTS A) \<and> A $ (p, \<gamma>, q) + d \<cdot> d' \<noteq> A $ (p, \<gamma>, q)"
+  using assms pre_star_rule_update_is_Init[OF assms]
+        pre_star_rule_update_spec'[OF assms(1), of "the_Ctr_Loc p" \<gamma> q]
+  by simp
+
+lemma inits_not_noninits: "p \<in> inits \<Longrightarrow> p \<in> noninits \<Longrightarrow> False"
+  unfolding inits_def noninits_def by auto
+
+lemma not_inits_is_noninits: "isols = {} \<Longrightarrow> p \<notin> inits \<Longrightarrow> p \<in> noninits"
+  unfolding inits_def noninits_def isols_def using state.exhaust_disc by auto
+
+definition pre_star_precondition :: "(('ctr_loc, 'noninit, 'label) state, 'label, 'weight) w_transitions \<Rightarrow> bool" where
+  "pre_star_precondition A \<equiv> (inits \<subseteq> LTS.srcs (wts_to_monoidLTS A) \<and> isols = {})"
+definition pre_star_invariant :: "(('ctr_loc, 'noninit, 'label) state, 'label, 'weight) w_transitions \<Rightarrow> bool" where
+  "pre_star_invariant A \<equiv> (isols = {})"
+ 
+lemma q_not_inits:
+  assumes "pre_star_precondition A"
+  assumes "A $ (p,\<gamma>,q) \<noteq> 0"
+  shows "q \<notin> inits"
+  using assms unfolding pre_star_precondition_def LTS.srcs_def wts_to_monoidLTS_def by auto
+
+lemma q_noninits:
+  assumes "pre_star_precondition A"
+  assumes "A $ (p,\<gamma>,q) \<noteq> 0"
+  shows "q \<in> noninits"
+  using q_not_inits[OF assms] assms(1) not_inits_is_noninits 
+  unfolding pre_star_precondition_def by presburger
+
+lemma 
+  assumes "pre_star_precondition A"
+      and "pre_star_rule A A'"
+      and "A' $ (p,\<gamma>,q) \<noteq> 0"
+      and "p \<in> noninits"
+    shows "q \<in> noninits"
+proof -
+  have "A $ (p,\<gamma>,q) = A' $ (p,\<gamma>,q)" using pre_star_rule_update_inits[OF assms(2)] assms(4) unfolding inits_def noninits_def by blast
+  then show ?thesis using assms(1,3) q_noninits by metis
+qed
+
+lemma 
+  assumes "pre_star_precondition A"
+  assumes "pre_star_rule A A'"
+  shows   "A' $ (p,\<gamma>,q) \<noteq> 0 \<and> A' $ (p,\<gamma>,q) \<noteq> 1 \<Longrightarrow> p \<in> inits"
+  using assms
+  oops
+
+lemma
+  assumes "inits \<subseteq> LTS.srcs (wts_to_monoidLTS A)"
+  shows   "accepts A (Noninit q, w) = 1"
+  using assms
+  oops
+
+lemma 
+  assumes "inits \<subseteq> LTS.srcs (wts_to_monoidLTS A)"
+  shows   "A $ (Init p, \<gamma>, Init p') \<le> pop_seq p \<gamma> p'"
+  using assms
+  oops
+
+definition word_of_trace :: "('ctr_loc, 'label) trace \<Rightarrow> 'label list" where
+  "word_of_trace t = map (fst) (snd t)"
+fun trace_to_pops :: "('ctr_loc, 'label) trace \<Rightarrow> ('ctr_loc \<times> 'label \<times> 'ctr_loc) list" where
+  "trace_to_pops (p,[]) = []"
+| "trace_to_pops (p,((\<gamma>,p')#xs)) = (p,\<gamma>,p')#(trace_to_pops (p',xs))"
+
+definition trace_pop_seq_sum :: "('ctr_loc, 'label) trace \<Rightarrow> 'weight" where
+  "trace_pop_seq_sum t = foldr (\<lambda>(p,\<gamma>,p') d. pop_seq p \<gamma> p' * d) (trace_to_pops t) 1"
+
+fun is_final_trace :: "('ctr_loc, 'noninit, 'label) final_trace \<Rightarrow> bool" where
+  "is_final_trace (pops,[]) = (Init (last pops) \<in> finals)"
+| "is_final_trace (_,t) = (Noninit (snd (List.last t)) \<in> finals)"
+
+definition word_of_final_trace :: "('ctr_loc, 'noninit, 'label) final_trace \<Rightarrow> 'label list" where
+  "word_of_final_trace ft = (word_of_trace (fst ft)) @ map (fst) (snd ft)"
+
+definition final_trace_accepts :: "('ctr_loc, 'noninit, 'label) final_trace \<Rightarrow> 'ctr_loc \<Rightarrow> 'label list \<Rightarrow> bool" where
+  "final_trace_accepts t p w \<equiv> is_final_trace t \<and> first (fst t) = p \<and> word_of_final_trace t = w" 
+
+fun noninit_trace_weight :: "'ctr_loc \<Rightarrow> ('label \<times> 'noninit) list \<Rightarrow> 'weight" where 
+  "noninit_trace_weight p [] = 1"
+| "noninit_trace_weight p ((\<gamma>,q)#qs) = 1" (* weight_of (p,\<gamma>,q)" *)
+
+definition final_trace_weight_sum :: "('ctr_loc, 'noninit, 'label) final_trace \<Rightarrow> 'weight" where
+  "final_trace_weight_sum ft = trace_pop_seq_sum (fst ft) * (noninit_trace_weight (last (fst ft)) (snd ft))"
+
+
+lemma "accepts A (p,w) = \<Sigma>{final_trace_weight_sum t | t::(('ctr_loc, 'noninit, 'label) final_trace). final_trace_accepts t p w}"
+  
+  (* Not quite enough... Need to look at path from (last t) to a final state *)
+  oops
 
 
 lemma lemma_3_1_w:
